src/Std/Data/DHashMap/Internal/WF.lean
@@ -983,7 +983,7 @@ theorem wfImp_filter [BEq α] [Hashable α] [EquivBEq α] [LawfulHashable α] {m
 
 /-! # `insertListₘ` -/
 
-theorem toListModel_insertListₘ [BEq α] [Hashable α] [EquivBEq α][LawfulHashable α]
+theorem toListModel_insertListₘ [BEq α] [Hashable α] [EquivBEq α] [LawfulHashable α]
     {m : Raw₀ α β} {l : List ((a : α) × β a)} (h : Raw.WFImp m.1) :
     Perm (toListModel (insertListₘ m l).1.buckets)
       (List.insertList (toListModel m.1.buckets) l) := by
@@ -994,6 +994,37 @@ theorem toListModel_insertListₘ [BEq α] [Hashable α] [EquivBEq α][LawfulHas
     simp only [insertListₘ, List.insertList]
     apply Perm.trans (ih (wfImp_insert h))
     apply List.insertList_perm_of_perm_first (toListModel_insert h) (wfImp_insert h).distinct
+
+/-! # `unionₘ` -/
+
+theorem insertMany_eq_insertListₘ_toListModel [BEq α] [Hashable α] (m m₂ : Raw₀ α β) :
+    insertMany m m₂.1 = insertListₘ m (toListModel m₂.1.buckets) := by
+  simp only [insertMany, bind_pure_comp, map_pure, bind_pure]
+  simp only [ForIn.forIn]
+  simp only [Raw.forIn_eq_forIn_toListModel, forIn_pure_yield_eq_foldl, Id.run_pure]
+  generalize toListModel m₂.val.buckets = l
+  suffices ∀ (t : { m' // ∀ (P : Raw₀ α β → Prop),
+    (∀ {m'' : Raw₀ α β} {a : α} {b : β a}, P m'' → P (m''.insert a b)) → P m → P m' }),
+      (List.foldl (fun m' p => ⟨m'.val.insert p.1 p.2, fun P h₁ h₂ => h₁ (m'.2 _ h₁ h₂)⟩) t l).val =
+    t.val.insertListₘ l from this _
+  intro t
+  induction l generalizing m with
+  | nil => simp [insertListₘ]
+  | cons hd tl ih =>
+    simp only [List.foldl_cons, insertListₘ]
+    apply ih
+
+theorem union_eq_unionₘ [BEq α] [Hashable α] (m₁ m₂ : Raw₀ α β) :
+    union m₁ m₂ = unionₘ m₁ m₂ := by
+  rw [union, unionₘ]
+  split <;> rw [insertMany_eq_insertListₘ_toListModel]
+
+theorem toListModel_unionₘ [BEq α] [Hashable α] [EquivBEq α] [LawfulHashable α]
+    {m₁ m₂ : Raw₀ α β} (h₁ : Raw.WFImp m₁.1) (h₂ : Raw.WFImp m₂.1) :
+    Perm (toListModel (unionₘ m₁ m₂).1.buckets)
+      (List.insertSmallerList (toListModel m₁.1.buckets) (toListModel m₂.1.buckets)) := by
+  rw [unionₘ, insertSmallerList, h₁.size_eq, h₂.size_eq]
+  split <;> exact toListModel_insertListₘ ‹_›
 
 end Raw₀
 
@@ -1133,6 +1164,22 @@ theorem toListModel_insertMany_list [BEq α] [Hashable α] [EquivBEq α] [Lawful
   rw [insertMany_eq_insertListₘ]
   apply toListModel_insertListₘ
   exact h
+
+/-! # `union` -/
+
+theorem wf_union₀ [BEq α] [Hashable α] [EquivBEq α] [LawfulHashable α]
+    {m₁ m₂ : Raw α β} {h₁ : 0 < m₁.buckets.size} {h₂ : 0 < m₂.buckets.size} (h'₁ : m₁.WF)
+    (h'₂ : m₂.WF) :
+    (Raw₀.union ⟨m₁, h₁⟩ ⟨m₂, h₂⟩).1.WF := by
+  rw [union]
+  split <;> exact wf_insertMany₀ ‹_›
+
+theorem toListModel_union [BEq α] [Hashable α] [EquivBEq α] [LawfulHashable α] {m₁ m₂ : Raw₀ α β}
+    (h₁ : Raw.WFImp m₁.1) (h₂ : Raw.WFImp m₂.1) :
+    Perm (toListModel (m₁.union m₂).1.buckets)
+      (List.insertSmallerList (toListModel m₁.1.buckets) (toListModel m₂.1.buckets)) := by
+  rw [union_eq_unionₘ]
+  exact toListModel_unionₘ h₁ h₂
 
 /-! # `Const.insertListₘ` -/
 
